cogent/llvm/checker/coq/Corres.v
@@ -2,10 +2,11 @@ From Coq Require Import List String ZArith.
 
 From ITree Require Import ITree ITreeFacts.
 
-From Vellvm Require Import LLVMAst LLVMEvents TopLevel Handlers InterpreterMCFG TopLevelRefinements DynamicTypes
-  CFG TypToDtyp InterpretationStack.
+From Vellvm Require Import LLVMAst LLVMEvents TopLevel Handlers InterpreterMCFG TopLevelRefinements
+  DynamicTypes CFG TypToDtyp InterpretationStack SymbolicInterpreter DenotationTheory ScopeTheory
+  DynamicValues ExpLemmas Scope.
 
-From Checker Require Import Denote Cogent Compiler Utils.Codegen Utils.Fail.
+From Checker Require Import Denote Cogent Compiler Utils.Codegen Utils.Fail Utils.Tactics.
 
 Import ListNotations.
 
@@ -17,9 +18,47 @@ Definition E_cfg : Type -> Type := CallE +' PickE +' UBE +' DebugE +' FailureE.
 Definition semantics_llvm_mcfg p : itree E_mcfg _ := model_to_L3 DTYPE_Void "main" [DV.UVALUE_I32 (DynamicValues.Int32.zero)] p.
 Definition semantics_llvm (p : vellvm_prog) : itree E_mcfg _ :=
   semantics_llvm_mcfg (convert_types (mcfg_of_tle p)).
+Notation "'interp_cfg'"  := interp_cfg3. 
+Notation "'interp_mcfg'" := interp_mcfg3. 
 
 Definition semantics_cogent (p : cogent_prog) : failT (itree E_mcfg) (memory * uval) := 
-  interp_cogent (denote_program p) "main" UUnit dummy_memory.
+  interp_cogent (denote_program p) "main" UUnit empty_memory.
+
+Section StateRel.
+
+  (* do things the helix way *)
+  Local Open Scope type_scope.
+
+  Definition state_cogent := memory.
+  Definition state_cogent_H := option memory.
+  Definition state_cogent_T (T : Type) := memory * T.
+  Definition state_cogent_OT (T : Type) := option (memory * T).
+
+  Definition state_cfg := memory_stack * (local_env * global_env).
+  Definition state_cfg_T (T : Type) := memory_stack * (local_env * (global_env * T)).
+  Definition state_cfg_res := state_cfg_T (block_id + uvalue).  
+  
+  Definition Rel_cfg : Type := state_cogent -> state_cfg -> Prop.
+  Definition Rel_cfg_T (A B : Type) : Type := state_cogent_T A -> state_cfg_T B -> Prop.
+  Definition Rel_cfg_OT (A B : Type) : Type := state_cogent_OT A -> state_cfg_T B -> Prop.
+
+  Definition lift_Rel_cfg {A B} (R : Rel_cfg) : Rel_cfg_T A B :=
+    fun '(c_mem, _) '(v_mem, (l, (g, _))) => R c_mem (v_mem, (l, g)).
+
+  Definition succ_rel_l {A B} (R : A -> B -> Prop) : option A -> B -> Prop :=
+    fun ma b => match ma with | Some a => R a b | _ => False end.
+  Definition succ_cfg {A B}: Rel_cfg_T A B -> Rel_cfg_OT A B := succ_rel_l.
+
+  Definition conj_rel {A B : Type} (R S: A -> B -> Prop): A -> B -> Prop :=
+    fun a b => R a b /\ S a b.
+
+  Record state_invariant (γ : ctx) (s : CodegenState) (cogent_mem : memory)
+                         (vellvm : state_cfg) : Prop :=
+  {}.
+
+End StateRel.
+
+Infix "⩕" := conj_rel (at level 85, right associativity).
 
 Section TopLevel.
 
@@ -35,7 +74,34 @@ Section TopLevel.
 
 End TopLevel.
 
+Import ExpTactics.
+
 Section Expressions.
+
+  Definition convert_uval (u : uval) : uvalue :=
+    match u with
+    | UPrim (LBool b) => UVALUE_I1 (Int1.repr (if b then 1 else 0))
+    | UPrim (LU8 w) => UVALUE_I8 (Int8.repr w)
+    | UPrim (LU32 w) => UVALUE_I32 (Int32.repr w)
+    | UPrim (LU64 w) => UVALUE_I64 (Int64.repr w)
+    | UUnit => UVALUE_I8 (Int8.repr 0)
+    end.
+
+  Definition compile_expr_res (v : texp typ) (γ : ctx) (s1 s2 : CodegenState) 
+                            : Rel_cfg_T uval (block_id * block_id + uvalue) :=
+    fun '(_, u) '(m,(l,(g,_))) =>
+      interp_cfg
+        (translate exp_to_instr (denote_exp (Some (typ_to_dtyp [] (fst v))) (convert_typ [] (snd v))))
+        g l m ≈ Ret (m, (l, (g, convert_uval u))).
+    
+
+  Record compile_expr_post (v : texp typ) (γ : ctx) (s1 s2 : CodegenState)
+                           (cogent_i: state_cogent) (vellvm_i : state_cfg)
+                           (cogent_f : state_cogent_T uval)
+                           (vellvm_f : state_cfg_T (block_id * block_id + uvalue)) : Prop :=
+  {
+    correct_result : compile_expr_res v γ s1 s2 cogent_f vellvm_f
+  }.
 
   Lemma compile_expr_correct :
     forall (s1 s2 : CodegenState) (v : texp typ)
@@ -43,12 +109,70 @@ Section Expressions.
            (next_blk blk prev_blk : block_id) (blks : ocfg typ)
            (g : global_env) (l : local_env) (vellvm_mem : memory_stack),
       compile_expr e next_blk s1 = inr (s2, (v, blk, blks)) ->
-        eutt
-          TT
+      state_invariant γ s1 cogent_mem (vellvm_mem, (l, g)) ->
+        eutt (
+          succ_cfg (
+            lift_Rel_cfg (state_invariant γ s1) ⩕ 
+            compile_expr_post v γ s1 s2 cogent_mem (vellvm_mem, (l, g))
+          ))
           (interp_expr (denote_expr γ e) cogent_mem)
-          (interp_cfg3 (denote_ocfg (convert_typ [] blks) (prev_blk, next_blk)) g l vellvm_mem).
+          (interp_cfg (denote_ocfg (convert_typ [] blks) (prev_blk, next_blk)) g l vellvm_mem).
   Proof.
-  Abort.
+    induction e; intros * COMPILE PRE.
+    -
+      cbn* in COMPILE; simp.
+      unfold denote_expr in *; cbn*.
+      unfold option_bind.
+      destruct (nth_error γ i).
+      + admit.
+      +
+    admit.
+    -
+    admit.
+    -
+      cbn* in COMPILE; simp.
+      unfold denote_expr in *; cbn*.
+      rewrite interp_expr_Ret.
+      rewrite denote_ocfg_unfold_not_in.
+      vred.
+      apply eutt_Ret; split; [| split]; cbn; eauto.
+      typ_to_dtyp_simplify.
+      unfold denote_exp; cbn.
+      go; reflexivity.
+      apply find_block_nil.
+    -
+      cbn* in COMPILE; simp.
+      unfold denote_expr in *; cbn*.
+      rewrite interp_expr_Ret.
+      rewrite denote_ocfg_unfold_not_in.
+      vred.
+      apply eutt_Ret; split; [| split]; cbn; eauto.
+      destruct l;
+        simpl;
+        typ_to_dtyp_simplify;
+        unfold denote_exp; cbn;
+        go; reflexivity.
+      apply find_block_nil.
+    - 
+      cbn* in COMPILE; simp.
+      rename e1 into bind, e2 into body.
+      rename l0 into bind_blks, l1 into body_blks.
+      rename b0 into body_entry.
+      unfold code_block.
+      rewrite convert_typ_ocfg_app.
+      rewrite denote_ocfg_app; eauto.
+      2: {
+        unfold no_reentrance.
+
+        
+        
+
+        
+
+      }
+
+      admit.
+  Qed.
 
 (* we want something like Lemma genNExpr_correct mixed with DSHAssign_correct *)
 
