cogent/llvm/checker/coq/Types.v
@@ -7,7 +7,7 @@ Open Scope Z_scope.
 Definition convert_num_type (t : num_type) : typ :=
   TYPE_I match t with
   | U8 => 8
-  | U16 => 16
+  (* | U16 => 16 *)
   | U32 => 32
   | U64 => 64
   end.
